nondeterministic_dataflow/BNA_Operators.thy
@@ -15,18 +15,18 @@ abbreviation "eos op p \<equiv> Write op p EOS"
 definition bna_feedback :: "('m + 'l, 'n + 'l, 'd) op \<Rightarrow> ('m, 'n, 'd) op" where
   "bna_feedback op = map_op projl projl (loop_op (case_sum (\<lambda>_. None) (Some o Inr)) (\<lambda>_. BEmpty) op)"
 
-corec (friend) cp_list where "cp_list \<pi> ps op = (case ps of p # ps \<Rightarrow> Read p (case_observation (Write (cp_list \<pi> ps op) (\<pi> p)) (cp_list \<pi> ps op) End) | [] \<Rightarrow> 
-  (case op of End \<Rightarrow> End | Write op p x \<Rightarrow> Write op p x | Read p f \<Rightarrow> Read p f))"
+corec (friend) cp_list where "cp_list \<pi> ps op = (case ps of p # ps \<Rightarrow> Read p (case_observation (Write (cp_list \<pi> ps op) (\<pi> p)) (cp_list \<pi> ps op) end_op) | [] \<Rightarrow> 
+  (case op of end_op \<Rightarrow> end_op | Write op p x \<Rightarrow> Write op p x | Read p f \<Rightarrow> Read p f))"
 
-lemma cp_list_code: "cp_list \<pi> ps op = (case ps of p # ps \<Rightarrow> Read p (case_observation (Write (cp_list \<pi> ps op) (\<pi> p)) (cp_list \<pi> ps op) End) | [] \<Rightarrow> op)"
+lemma cp_list_code: "cp_list \<pi> ps op = (case ps of p # ps \<Rightarrow> Read p (case_observation (Write (cp_list \<pi> ps op) (\<pi> p)) (cp_list \<pi> ps op) end_op) | [] \<Rightarrow> op)"
   by (subst cp_list.code) (auto split: list.splits op.splits)
 
 corec bna_identity :: "('m :: enum, 'm, 'd) op" where
-  "bna_identity = (case Enum.enum :: 'm list of (p # ps) \<Rightarrow> Read p (case_observation (Write (cp_list id ps bna_identity) p) (cp_list id ps bna_identity) End))"
+  "bna_identity = (case Enum.enum :: 'm list of (p # ps) \<Rightarrow> Read p (case_observation (Write (cp_list id ps bna_identity) p) (cp_list id ps bna_identity) end_op))"
 
 corec bna_transpose :: "('m :: enum + 'n :: enum, 'n + 'm, 'd) op" where
   "bna_transpose = (case Enum.enum :: 'm list of (p # ps) \<Rightarrow>
-  Read (Inl p) (case_observation (Write (cp_list (case_sum Inr Inl) (map Inl ps @ map Inr Enum.enum) bna_transpose) (Inr p)) bna_transpose End))"
+  Read (Inl p) (case_observation (Write (cp_list (case_sum Inr Inl) (map Inl ps @ map Inr Enum.enum) bna_transpose) (Inr p)) bna_transpose end_op))"
 
 abbreviation "bna_parcomp \<equiv> pcomp_op"
 abbreviation "bna_seqcomp \<equiv> scomp_op"
